Kraken/Theorems.lean
@@ -3,6 +3,7 @@ Kraken - Helper Theorems
 -/
 
 import Kraken.Semantics
+import Kraken.Syntax
 
 -- UInt64.ofInt (k : Int) ≠ 0 when k is a natural number with k < 2^64 and k ≠ 0
 -- This proof uses only core Lean lemmas (no Batteries/Mathlib)
@@ -23,3 +24,51 @@ theorem UInt64_ofInt_natCast_ne_zero (k : Nat) (h_lt : k < 2^64) (h_ne : k ≠ 0
   have hzero : (0 : Nat) % 2^64 = 0 := Nat.zero_mod (2^64)
   rw [h2, hkmod, hzero] at h1
   exact h_ne h1
+
+theorem simpleAlignedStore64 (s : MachineData) (addr : BitVec 64) (v : BitVec 64) (ret: MachineData → Effects)
+  (hAligned: addr % 8 = 0)
+  (hContains: UInt64.ofBitVec addr ∈ s.dmem):
+  MachineData.store s addr v ret =
+  require_write_access addr Width.W64 (fun _unit =>
+    ret { s with dmem := s.dmem.insert (UInt64.ofBitVec addr) (UInt64.ofBitVec v) }) :=
+by
+  simp only [MachineData.store,Width.bytesv,Width.bytes]
+  have: addr % 8#64 = 0#64 := by grind
+  simp only [this]
+  have: UInt64.ofBitVec (addr &&& ~~~0b111#64) = UInt64.ofBitVec addr := by
+    bv_decide
+  rw [this]
+  have: addr &&& 7#64 = 0 := by bv_decide
+  simp [this,Width.bits]
+  -- TODO: lift and generalize this
+  have (old v: BitVec 64): BitVec.replace old 0 v = v := by
+    simp [BitVec.replace,BitVec.drop]
+    bv_decide
+  simp [this]
+  rw [Std.ExtHashMap.getElem?_eq_some_getElem! hContains]
+
+-- AE, JP: it would be nice to eliminate CPS from the post and say that the post
+-- is just called with the value that is loaded
+theorem simpleAlignedLoad64 (s : MachineData) (addr : BitVec 64) (ret: BitVec 64 → MachineData → Effects)
+  (hAligned: addr % 8 = 0)
+  (hContains: UInt64.ofBitVec addr ∈ s.dmem):
+  MachineData.load s addr .W64 ret =
+  require_read_access addr Width.W64 (fun _unit =>
+    ret (s.dmem[UInt64.ofBitVec addr]!.toBitVec) s) :=
+by
+  simp only [MachineData.load,Width.bytesv,Width.bytes]
+  -- TODO: figure out why `simp` cannot deduce the fact below; setting
+  -- pp.coercions to false reveals that one version of the lemma uses
+  -- `OfNat.ofNat` to produce a BitVec, while the other uses `OfNat.ofNat` to
+  -- produce a Nat, followed by a call to `BitVec.ofNat`, and there appears to
+  -- be no simp-rule that would show that one can be rewritten into the other.
+  have: addr % 8#64 = 0#64 := by grind
+  simp only [this]
+  -- TODO: perhaps there should be a rule for this that can be in a simpset or a
+  -- grindset to facilitate this sort of reasoning
+  have: UInt64.ofBitVec (addr &&& ~~~0b111#64) = UInt64.ofBitVec addr := by
+    bv_decide
+  rw [this]
+  have: addr &&& 7#64 = 0 := by bv_decide
+  simp [this,Width.bits]
+  rw [Std.ExtHashMap.getElem?_eq_some_getElem! hContains]
